complete ex1_down

theories/opt/ex1_down.v
@@ -1,4 +1,4 @@
-From stbor.sim Require Import local invariant refl_step.
+From stbor.sim Require Import local invariant refl.
 From stbor.sim Require Import tactics simple program.
 From stbor.sim Require Import refl_step right_step left_step derived_step viewshift.
 
@@ -7,7 +7,7 @@ Set Default Proof Using "Type".
 (** Moving a read of a mutable reference down across code that *may* use that ref. *)
 
 (* Assuming x : &mut i32 *)
-Definition ex1_down : function :=
+Definition ex1_down_unopt : function :=
   fun: ["i"],
     let: "x" := new_place (&mut int) "i" in (* put argument into place *)
     retag_place "x" (RefPtr Mutable) int FnEntry ;;
@@ -27,7 +27,7 @@ Definition ex1_down_opt : function :=
     "v"
   .
 
-Lemma ex1_down_sim_fun : ⊨ᶠ ex1_down ≥ ex1_down_opt.
+Lemma ex1_down_sim_fun : ⊨ᶠ ex1_down_unopt ≥ ex1_down_opt.
 Proof.
   (* We can't use sim_simple because we need to track our stack frame id *)
   intros fs ft LOOK rarg es et vls vlt σs σt FREL SUBSTs SUBSTt.
@@ -60,10 +60,10 @@ Proof.
     sim_apply sim_body_retag_ref_fn_entry; [simpl; lia|eauto| |done|..].
     { rewrite -cmra_assoc (cmra_comm (res_cs _ _)) cmra_assoc. eauto. }
     { eapply arel_mono; [done|..|exact AREL]. solve_res. } clear VALID.
-    move=> l' told tnew hplt α' nxtp' r0 ? _ IS_i σs2 σt2 s_new tk _ /=.
+    move=> l' told tnew hplt α' nxtp' r0 ? _ IS_i InD σs2 σt2 s_new tk _ /=.
     subst sarg.
-    specialize (IS_i O ltac:(simpl; lia)). rewrite shift_loc_0_nat in IS_i.
-    destruct IS_i as [(ss & st & IS_i & Eqss & Eqst & ARELs) TOP].
+    have IS_O := (IS_i O ltac:(simpl; lia)). rewrite shift_loc_0_nat in IS_O.
+    destruct IS_O as [(ss & st & Eql' & Eqss & Eqst & ARELs) TOP].
     rewrite insert_empty.
     (* Write local *)
     sim_apply sim_body_write_local_1; [solve_sim..|].
@@ -92,16 +92,60 @@ Proof.
   sim_apply_r sim_body_deref_r =>/=.
   sim_apply_r sim_body_copy_protected_r;
     [solve_sim..|by rewrite lookup_insert|by eapply elem_of_dom_2|].
-  apply: sim_body_result=>_ /=.
+  intros Eqss3 Eqst3.
+  apply: sim_body_result=> Hval /=.
   apply: sim_body_let_r=>/=.
   (* Free stuff *)
   sim_apply sim_body_free_unique_local_1;
     [done|rewrite /res_loc /= insert_empty; solve_sim |by left|].
-  simpl => _ _ α4 _.
+  move => _ _ α4 _ σs4 σt4.
   sim_apply sim_body_let=>/=.
+  (* Remove protection *)
+  set r1 := rarg ⋅ r0 ⋅ res_cs (snc σt) {[tnew := dom (gset loc) hplt]} ⋅
+              res_tag tnew tk hplt ⋅ rf'.
+  set r2 := rarg ⋅ r0 ⋅ res_cs (snc σt) ∅ ⋅ res_tag tnew tk hplt ⋅ rf'.
+  rewrite (_: rarg ⋅ res_cs (snc σt) {[tnew := dom (gset loc) hplt]} ⋅
+              res_tag tnew tk hplt ⋅ r0 ⋅ rf' ≡ r1); last first.
+  { rewrite -cmra_assoc (cmra_comm r0 rf') cmra_assoc (cmra_comm _ r0)
+            !cmra_assoc (cmra_comm r0) //. }
+  apply (viewshift_state_sim_local_body _ _ _ _ r1 r2).
+  { rewrite /r1 /r2. do 2 apply viewshift_state_frame_r.
+    rewrite -insert_empty. apply vs_state_drop_protector; [done|].
+    move => l1 /InD [i [/= Lti ?]]. subst l1.
+    destruct i; [|clear -Lti; by lia]. rewrite shift_loc_0_nat.
+    move => ss4 /= /lookup_delete_Some [? Eqst4].
+    rewrite Eqst4 in Eqst3. simplify_eq. exists ss.
+    rewrite lookup_delete_ne; [|done]. split; [done|].
+    move : ARELs. apply arel_mono; [|solve_res]. clear -Hval.
+    apply (cmra_valid_included _ _ Hval).
+    do 2 (etrans; [|apply cmra_included_l]).
+    apply cmra_mono_r. solve_res. } clear Hval.
   (* Finishing up. *)
   apply: sim_body_result => Hval. split.
-  - exists σt.(snc). split; [done|]. admit.
+  - exists σt.(snc). split; [done|]. rewrite /end_call_sat.
+    apply (cmap_lookup_op_unique_included (res_cs (snc σt) ∅).(rcm));
+      [apply Hval|apply prod_included; rewrite /r2; solve_res|..].
+    by rewrite res_cs_lookup.
   - constructor; [|by constructor].
-    move : ARELs. apply arel_mono; [done|solve_res].
-Abort.
+    move : ARELs. rewrite /r2. apply arel_mono; [done|solve_res].
+Qed.
+
+(** Top-level theorem: Two programs that only differ in the
+"ex1_down" function are related. *)
+Corollary ex1_down (prog: fn_env) :
+  stuck_decidable →
+  prog_wf prog →
+  let prog_src := <["ex1_down":=ex1_down_unopt]> prog in
+  let prog_tgt := <["ex1_down":=ex1_down_opt]> prog in
+  behave_prog prog_tgt <1= behave_prog prog_src.
+Proof.
+  intros Hdec Hwf. apply sim_prog_sim_classical.
+  { apply Hdec. }
+  { apply has_main_insert, Hwf; done. }
+  apply sim_mod_funs_local.
+  apply sim_mod_funs_insert; first done.
+  - exact: ex1_down_sim_fun.
+  - exact: sim_mod_funs_refl.
+Qed.
+
+Print Assumptions ex1_down.
